external/Goose/github_com/mit_pdos/go_nfsd/kvs.v
@@ -33,11 +33,11 @@ Definition KVS__MultiPut: val :=
   rec: "KVS__MultiPut" "kvs" "pairs" :=
     let: "op" := jrnl.Begin (struct.loadF KVS "log" "kvs") in
     ForSlice (struct.t KVPair) <> "p" "pairs"
-      (if: (struct.get KVPair "Key" "p" ≥ struct.loadF KVS "sz" "kvs") || (struct.get KVPair "Key" "p" < common.LOGSIZE)
+      ((if: (struct.get KVPair "Key" "p" ≥ struct.loadF KVS "sz" "kvs") || (struct.get KVPair "Key" "p" < common.LOGSIZE)
       then Panic "oops"
       else #());;
       let: "akey" := addr.MkAddr (struct.get KVPair "Key" "p") #0 in
-      jrnl.Op__OverWrite "op" "akey" common.NBITBLOCK (struct.get KVPair "Val" "p");;
+      jrnl.Op__OverWrite "op" "akey" common.NBITBLOCK (struct.get KVPair "Val" "p"));;
     let: "ok" := jrnl.Op__CommitWait "op" #true in
     "ok".
 
