external/Goose/github_com/mit_pdos/gokv/pb/controller.v
@@ -45,9 +45,9 @@ Definition ControllerServer__HandleFailedReplicas: val :=
     let: "n" := slice.len (struct.loadF pb.Configuration "Replicas" (struct.loadF ControllerServer "conf" "s")) - MapLen (struct.loadF ControllerServer "failed" "s") in
     let: "newReplicas" := ref_to (slice.T uint64T) (NewSliceWithCap uint64T #0 "n") in
     ForSlice uint64T "i" "r" (struct.loadF pb.Configuration "Replicas" (struct.loadF ControllerServer "conf" "s"))
-      (if: ~ (Fst (MapGet (struct.loadF ControllerServer "failed" "s") "i"))
+      ((if: ~ (Fst (MapGet (struct.loadF ControllerServer "failed" "s") "i"))
       then "newReplicas" <-[slice.T uint64T] SliceAppend uint64T (![slice.T uint64T] "newReplicas") "r"
-      else #());;
+      else #()));;
     struct.storeF ControllerServer "conf" "s" (struct.new pb.Configuration [
       "Replicas" ::= ![slice.T uint64T] "newReplicas"
     ]);;
@@ -75,14 +75,14 @@ Definition ControllerServer__HeartbeatThread: val :=
       struct.storeF ControllerServer "failed" "s" (NewMap boolT #());;
       ForSlice ptrT "i" <> "clerks"
         (let: "i" := "i" in
-        SliceSet ptrT "hbtimers" "i" (time.AfterFunc "HBTIMEOUT" (λ: <>,
+        SliceSet ptrT "hbtimers" "i" (time.AfterFunc "HBTIMEOUT" ((λ: <>,
           lock.acquire (struct.loadF ControllerServer "mu" "s");;
           (if: (struct.loadF ControllerServer "cn" "s" = "cn")
           then MapInsert (struct.loadF ControllerServer "failed" "s") "i" #true
           else #());;
           lock.release (struct.loadF ControllerServer "mu" "s");;
           #()
-          )));;
+          ))));;
       Skip;;
       (for: (λ: <>, #true); (λ: <>, Skip) := λ: <>,
         lock.acquire (struct.loadF ControllerServer "mu" "s");;
@@ -141,12 +141,12 @@ Definition StartControllerServer: val :=
     ]);;
     Fork (ControllerServer__HeartbeatThread "s");;
     let: "handlers" := NewMap ((slice.T byteT -> ptrT -> unitT)%ht) #() in
-    MapInsert "handlers" CONTROLLER_ADD (λ: "raw_args" <>,
+    MapInsert "handlers" CONTROLLER_ADD ((λ: "raw_args" <>,
       let: "dec" := marshal.NewDec "raw_args" in
       let: "newServer" := marshal.Dec__GetInt "dec" in
       ControllerServer__AddNewServerRPC "s" "newServer";;
       #()
-      );;
+      ));;
     let: "r" := urpc.MakeServer "handlers" in
     urpc.Server__Serve "r" "me";;
     #().
